More refactoring for sharing Clocks

Clocks.v
@@ -1,4 +1,5 @@
 Require Import Velus.Common.
+Require Import List.
 
 Module Type CLOCKS
        (Ids : IDS).
@@ -9,6 +10,112 @@ Module Type CLOCKS
   | Cbase : clock                            (* base clock *)
   | Con   : clock -> ident -> bool -> clock. (* subclock *)
 
+  Inductive Is_free_in_clock : ident -> clock -> Prop :=
+  | FreeCon1:
+      forall x ck' xc,
+        Is_free_in_clock x (Con ck' x xc)
+  | FreeCon2:
+      forall x y ck' xc,
+        Is_free_in_clock x ck'
+        -> Is_free_in_clock x (Con ck' y xc).
+  
+  (** ** Well-clocking *)
+
+  Inductive wc_clock (vars: list (ident * clock)) : clock -> Prop :=
+  | CCbase:
+      wc_clock vars Cbase
+  | CCon:
+      forall ck x b,
+        wc_clock vars ck ->
+        In (x, ck) vars ->
+        wc_clock vars (Con ck x b).
+
+  Definition wc_env vars : Prop :=
+    Forall (fun xck => wc_clock vars (snd xck)) vars.
+
+  Lemma wc_env_var:
+    forall vars x ck,
+      wc_env vars
+      -> In (x, ck) vars
+      -> wc_clock vars ck.
+  Proof.
+    intros vars x ck Hwc Hcv.
+    now apply In_Forall with (2:=Hcv) in Hwc.
+  Qed.
+
+  Lemma wc_clock_add:
+    forall x v env ck,
+      ~InMembers x env ->
+      wc_clock env ck ->
+      wc_clock ((x, v) :: env) ck.
+  Proof.
+    induction ck; auto using wc_clock.
+    inversion 2.
+    auto using wc_clock with datatypes.
+  Qed.
+  
+  Lemma wc_env_add:
+    forall x env ck,
+      ~InMembers x env ->
+      wc_clock env ck ->
+      wc_env env ->
+      wc_env ((x, ck) :: env).
+  Proof.
+    intros ** Hnm Hwc Hwce.
+    constructor.
+    now apply wc_clock_add; auto.
+    apply all_In_Forall.
+    destruct x0 as (x' & ck').
+    intro Hin.
+    apply In_Forall with (1:=Hwce) in Hin.
+    apply wc_clock_add; auto.
+  Qed.
+
+  Lemma wc_clock_sub:
+    forall vars ck x b,
+      wc_env vars
+      -> wc_clock vars (Con ck x b)
+      -> In (x, ck) vars.
+  Proof.
+    intros vars ck x b Hwc Hclock.
+    inversion_clear Hclock as [|? ? ? Hclock' Hcv'].
+    assumption.
+  Qed.
+
+  Require Import Morphisms.
+  Import Permutation.
+
+  Instance wc_clock_Proper:
+    Proper (@Permutation (ident * clock) ==> @eq clock ==> iff) wc_clock.
+  Proof.
+    intros env' env Henv ck' ck Hck.
+    rewrite Hck; clear Hck ck'.
+    induction ck.
+    - split; auto using wc_clock.
+    - destruct IHck.
+      split; inversion_clear 1; constructor;
+        try rewrite Henv in *;
+        auto using wc_clock.
+  Qed.
+
+  Instance wc_env_Proper:
+    Proper (@Permutation (ident * clock) ==> iff) wc_env.
+  Proof.
+    intros env' env Henv.
+    unfold wc_env.
+    split; intro HH.
+    - apply all_In_Forall.
+      intros x Hin.
+      rewrite <-Henv in Hin.
+      apply In_Forall with (1:=HH) in Hin.
+      now rewrite Henv in Hin.
+    - apply all_In_Forall.
+      intros x Hin.
+      rewrite Henv in Hin.
+      apply In_Forall with (1:=HH) in Hin.
+      now rewrite <-Henv in Hin.
+  Qed.
+  
   (** ** Parent relation *)
   
   Inductive clock_parent ck : clock -> Prop :=
@@ -70,6 +177,15 @@ Module Type CLOCKS
     apply clock_parent_not_refl with (1:=Hck).
   Qed.
 
+  Lemma clock_no_loops:
+    forall ck x b,
+      Con ck x b <> ck.
+  Proof.
+    induction ck as [|? IH]; [discriminate 1|].
+    injection 1; intros ? Heq.
+    apply IH.  
+  Qed.
+
   Lemma clock_parent_Con:
     forall ck ck' i b j c,
       clock_parent (Con ck i b) (Con ck' j c)
@@ -113,6 +229,41 @@ Module Type CLOCKS
     intros ck x b Hp; apply clock_parent_strict with (1:=Hp); constructor.
   Qed.
 
+  Lemma Is_free_in_clock_self_or_parent:
+    forall x ck,
+      Is_free_in_clock x ck
+      -> exists ck' b, ck = Con ck' x b \/ clock_parent (Con ck' x b) ck.
+  Proof.
+    Hint Constructors clock_parent.
+    induction ck as [|? IH]; [now inversion 1|].
+    intro Hfree.
+    inversion Hfree as [|? ? ? ? Hfree']; clear Hfree; subst.
+    - exists ck, b; now auto.
+    - specialize (IH Hfree'); clear Hfree'.
+      destruct IH as [ck' [b' Hcp]].
+      exists ck', b'; right.
+      destruct Hcp as [Hcp|Hcp]; [rewrite Hcp| inversion Hcp]; now auto.
+  Qed.
+
+  Lemma wc_clock_parent:
+    forall C ck' ck,
+      wc_env C
+      -> clock_parent ck ck'
+      -> wc_clock C ck'
+      -> wc_clock C ck.
+  Proof.
+    Hint Constructors wc_clock.
+    induction ck' as [|ck' IH]; destruct ck as [|ck i' ty' b'];
+    try now (inversion 3 || auto).
+    intros Hwc Hp Hck.
+    inversion Hp as [j c [HR1 HR2 HR3]|ck'' j c Hp' [HR1 HR2 HR3]].
+    - rewrite <-HR1 in *; clear HR1 HR2 HR3.
+      now inversion_clear Hck.
+    - subst.
+      apply IH with (1:=Hwc) (2:=Hp').
+      now inversion Hck.
+  Qed.
+    
 End CLOCKS.
 
 Module ClocksFun (Ids : IDS) <: CLOCKS Ids.
